\documentclass{article}
\usepackage[utf8]{inputenc}
\usepackage{amsmath}
\usepackage{multicol}

\begin{document}

$$(\exists n \in \mathbb{N})[2+2^{2}+2^{3}+...+2^{n}=2^{n+1}-2]$$
Proof: By induction.
\newline
$n=1$:
\begin{align*}
2&=2^{1+1}-2\\
2&=2^{2}-2\\
2&=2
\end{align*}
\newline
Assume $n=k$ holds:
$$2+2^{2}+2^{3}+...+2^{k}=2^{k+1}-2$$
Show that $n=k+1$ holds
\begin{equation*}
2+2^{2}+2^{3}+...+2^{k}+2^{k+1}=2^{(k+1)+1}-2 \tag*{(By induction)}
\end{equation*}
\begin{align*}
2+2^{2}+2^{3}+...+2^{k}+2^{k+1}&=2^{k+1}-2+2^{k+1}\\
&=2*2^{k}-2+2*2^{k}\\
&=4*2^{k}-2\\
&=2^2*2^{k}-2\\
&=2^{k+2}-2
\end{align*}
Therefore by induction the equation holds for all $n$.
\newline
QED.

\end{document}